src/ocaml/hipparser.ml
@@ -7,6 +7,17 @@ open Extraction.HiFirrtl
 open Extraction.ExpandConnects_inst 
 open Extraction.ExpandWhens_inst
 
+let () =
+  (* 调整 GC 参数，减小 Major GC 频率，提高性能 *)
+  let open Gc in
+  let c = get () in
+  set { c with
+    minor_heap_size = 64 * 1024 * 1024;  (* minor heap 大小，默认 256KB，增大到 4MB *)
+    major_heap_increment = 256;         (* major heap 每次增长量，默认 128，增大到 256 *)
+    space_overhead = 180;               (* 允许的空间开销百分比，默认 80，适当放宽 *)
+    max_overhead = 500;
+    allocation_policy = 2;   (* First-fit 分配策略 *)}
+
 let args = [
   ]
 
@@ -30,12 +41,9 @@ let whitelist = ["w"; "out"]
 let expr = Mast.Eprim_binop (Ast.Bmul, "y", "out")*)
 
 let anon file =
-  (*let result = Compare_conn_map.expand map whitelist expr in
-  Compare_conn_map.pp_expr stdout result;*)
-
   (* mlir connection tree *)
   let mlir_file = fir_to_mlir file in
-  let mlirf = Mparser.mlirparse mlir_file in 
+  let mlirf = Mparser.mlirparse mlir_file in output_string stdout "mlir\n";
   (*Mast.pp_modules stdout mlirf;
   output_string stdout "\nfirtool connection tree\n";*)
   let mlir_cm = Mast.cm_modl mlirf Mast.initmap_s in 
@@ -45,36 +53,46 @@ let anon file =
 
   (* ocaml connection tree *)
   let hif_ast = Parser.hiparse file in 
-  let oc_fir = (*open_out (Transhiast.process_string in_file "_cons.txt"*) stdout in
-  
+  let oc_fir = open_out (Transhiast.process_string file "_res.fir") in
+
   let ((modmap, _), map) = Transhiast_without_inline.mapcir hif_ast in 
   let hif_without_inline = Transhiast_without_inline.trans_cir hif_ast modmap map in
   (*output_string oc_fir "\norigin\n";
-  Printfir.pp_fcircuit_fir oc_fir hif_without_inline;
+  Printfir.pp_fcircuit_fir oc_fir hif_without_inline;*)
+  let ut0 = (Unix.times()).tms_utime in 
+  match preprocess_subaccess hif_without_inline with
+  | Some fcir -> let ut1 = (Unix.times()).tms_utime in 
+    (*output_string oc_fir "\npreprocess subaccess\n";
+    Printfir.pp_fcircuit_fir oc_fir fcir;*)
+    printf "preprocess subaccess time : %f\n" (Float.sub ut1 ut0); 
 
-  output_string oc_fir "\nafter expandconnects :\n";*)
-  (match expandconnects hif_without_inline with
-  | Some c_expandconnects -> (*Printfir_pair.pp_fcircuit_fir oc_fir c_expandconnects;
+  (match expandconnects fcir with
+  | Some c_expandconnects -> let ut2 = (Unix.times()).tms_utime in 
+    (*output_string oc_fir "\nafter expandconnects :\n";
+    Printfir_pair.pp_fcircuit_fir oc_fir c_expandconnects;
     output_string oc_fir "\nafter expandwhens :\n";*)
+    printf "expandConnects time : %f\n" (Float.sub ut2 ut1); 
     (match expandWhens c_expandconnects with
-    | Some ((c_expandwhens, conn_map), pvlist) -> (*Printfir_pair.pp_fcircuit_fir oc_fir c_expandwhens;*)
-    (* compare conn_map between mlir and ocaml *)
-      Mast.StringMap.iter (fun mv mod_cm -> output_string stdout ("\nmodule "^mv^" :\n");
+    | Some ((c_expandwhens, conn_map), pvlist) -> let ut3 = (Unix.times()).tms_utime in 
+      (*Printfir_pair.pp_fcircuit_fir oc_fir c_expandwhens;*)
+      printf "expandWhens time : %f\n" (Float.sub ut3 ut2); 
+      (* compare conn_map between mlir and ocaml *)
+      (*Mast.StringMap.iter (fun mv mod_cm -> output_string stdout ("\nmodule "^mv^" :\n");
         let modnum = Mast.StringMap.find mv modmap in
         let ((map0, map1), tmap) = Mast.StringMap.find mv map in 
         let modnump = Obj.magic (modnum, 0) in
         match PVM.find modnump conn_map with
         | Some ocaml_mod_cm -> match PVM.find modnump pvlist with
           | Some mod_pvlist -> 
-            let whitelist = List.map (fun pv -> Compare_conn_map.pair_to_string (Obj.magic pv) map1 tmap) mod_pvlist in 
-            Compare_conn_map.compare_ocaml_mlir (PVM.elements ocaml_mod_cm) ocaml_mod_cm mod_pvlist map1 tmap mod_cm whitelist
+            (*let whitelist = List.map (fun pv -> Compare_conn_map.pair_to_string (Obj.magic pv) map1 tmap) mod_pvlist in 
+            Compare_conn_map.compare_ocaml_mlir (PVM.elements ocaml_mod_cm) ocaml_mod_cm mod_pvlist map1 tmap mod_cm whitelist*)();
           | _ -> output_string stdout ("find module "^mv^" in whitelist error\n");
         | _ -> output_string stdout ("find module "^mv^" in ocaml cm error\n");
-        ) mlir_cm; 
+        ) mlir_cm; *)
 
     | None -> output_string stdout "error expandwhens\n";)
-  | None -> output_string stdout "error expandconnects\n";)
-
+  | None -> output_string stdout "error expandconnects\n";) 
+  | None -> output_string stdout "error subaccess preprocess\n"
   (*let map_p2s = Transhiast.StringMap.fold (fun key ft acc -> let base_num = Obj.magic (Stdlib.List.hd (Stdlib.List.rev (Transhiast.StringMap.find key map0))) in
         Pair2string.store_pair key 0 base_num ft acc) tmap_ast Transhiast.IntPairMap.empty in
 
